qed most of `evidence`, except another issue with serde inj;
see `wish_evidVrf_sig_pred`

new/proof/github_com/sanjit_bhat/pav/client_proof/evidence.v
@@ -3,15 +3,299 @@ From New.proof.github_com.sanjit_bhat.pav Require Import prelude.
 
 From New.proof Require Import bytes.
 From New.proof.github_com.sanjit_bhat.pav Require Import
-  cryptoffi ktcore.
+  cryptoffi ktcore safemarshal.
 
 From New.proof.github_com.sanjit_bhat.pav.client_proof Require Import
   base.
 
 Module client.
 Import base.client.
+
+Module evidVrf.
+Record t :=
+  mk' {
+    vrfPk0: list w8;
+    sig0: list w8;
+    vrfPk1: list w8;
+    sig1: list w8;
+  }.
+
 Section proof.
 Context `{hG: heapGS Σ, !ffi_semantics _ _, !globalsGS Σ} {go_ctx : GoContext}.
+
+Definition own ptr obj d : iProp Σ :=
+  ∃ sl_vrfPk0 sl_sig0 sl_vrfPk1 sl_sig1,
+  "Hstruct" ∷ ptr ↦{d} (client.evidVrf.mk sl_vrfPk0 sl_sig0 sl_vrfPk1 sl_sig1) ∗
+
+  "Hsl_vrfPk0" ∷ sl_vrfPk0 ↦*{d} obj.(vrfPk0) ∗
+  "Hsl_sig0" ∷ sl_sig0 ↦*{d} obj.(sig0) ∗
+  "Hsl_vrfPk1" ∷ sl_vrfPk1 ↦*{d} obj.(vrfPk1) ∗
+  "Hsl_sig1" ∷ sl_sig1 ↦*{d} obj.(sig1).
+
+End proof.
+End evidVrf.
+
+Module evidLink.
+Record t :=
+  mk' {
+    epoch: w64;
+    link0: list w8;
+    sig0: list w8;
+    link1: list w8;
+    sig1: list w8;
+  }.
+
+Section proof.
+Context `{hG: heapGS Σ, !ffi_semantics _ _, !globalsGS Σ} {go_ctx : GoContext}.
+
+Definition own ptr obj d : iProp Σ :=
+  ∃ sl_link0 sl_sig0 sl_link1 sl_sig1,
+  "Hstruct" ∷ ptr ↦{d} (client.evidLink.mk obj.(epoch) sl_link0 sl_sig0 sl_link1 sl_sig1) ∗
+
+  "Hsl_link0" ∷ sl_link0 ↦*{d} obj.(link0) ∗
+  "Hsl_sig0" ∷ sl_sig0 ↦*{d} obj.(sig0) ∗
+  "Hsl_link1" ∷ sl_link1 ↦*{d} obj.(link1) ∗
+  "Hsl_sig1" ∷ sl_sig1 ↦*{d} obj.(sig1).
+
+End proof.
+End evidLink.
+
+Module Evid.
+Record t :=
+  mk' {
+    vrf: option evidVrf.t;
+    link: option evidLink.t;
+  }.
+
+Section proof.
+Context `{hG: heapGS Σ, !ffi_semantics _ _, !globalsGS Σ} {go_ctx : GoContext}.
+
+Definition own ptr obj d : iProp Σ :=
+  ∃ ptr_vrf ptr_link,
+  "Hstruct" ∷ ptr ↦{d} (client.Evid.mk ptr_vrf ptr_link) ∗
+
+  "Hown_vrf" ∷
+    match obj.(vrf) with
+    | Some vrf => evidVrf.own ptr_vrf vrf d
+    | None => ⌜ptr_vrf = null⌝
+    end ∗
+  "Hown_link" ∷
+    match obj.(link) with
+    | Some link => evidLink.own ptr_link link d
+    | None => ⌜ptr_link = null⌝
+    end.
+
+End proof.
+End Evid.
+
+Section proof.
+Context `{hG: heapGS Σ, !ffi_semantics _ _, !globalsGS Σ} {go_ctx : GoContext}.
+
+(* TODO: move these into sep file. *)
+Class sigG Σ := {
+  #[local] vrf_inG :: ghost_varG Σ (list w8);
+  #[local] links_inG :: mono_listG (list w8) Σ;
+}.
+Context `{sigG Σ}.
+
+Record sig_names :=
+  mk {
+    vrf_name : gname;
+    links_name : gname;
+  }.
+Context {sigγ : sig_names}.
+
+Definition sig_pred_vrf γ enc : iProp Σ :=
+  ∃ vrfPk,
+  "%Henc" ∷ ⌜enc = ktcore.VrfSig.pure_enc (ktcore.VrfSig.mk' (W8 ktcore.VrfSigTag) vrfPk)⌝ ∗
+  "#Hshot" ∷ ghost_var γ (□) vrfPk.
+
+Definition sig_pred_links γ enc : iProp Σ :=
+  (* TODO: add map invs once figure out partial-epoch adtr. *)
+  ∃ ep link links,
+  "%Henc" ∷ ⌜enc = ktcore.LinkSig.pure_enc (ktcore.LinkSig.mk' (W8 ktcore.LinkSigTag) ep link)⌝ ∗
+  "#Hlb" ∷ mono_list_lb_own γ links ∗
+  "%Hlook" ∷ ⌜links !! uint.nat ep = Some link⌝.
+
+Definition sig_pred γ enc : iProp Σ :=
+  sig_pred_vrf γ.(vrf_name) enc ∨ sig_pred_links γ.(links_name) enc.
+
+#[global] Instance sig_pred_pers γ e : Persistent (sig_pred γ e).
+Proof. apply _. Qed.
+
+Definition wish_evidVrf e pk : iProp Σ :=
+  "#Hwish0" ∷ ktcore.wish_VerifyVrfSig pk e.(evidVrf.vrfPk0) e.(evidVrf.sig0) ∗
+  "#Hwish1" ∷ ktcore.wish_VerifyVrfSig pk e.(evidVrf.vrfPk1) e.(evidVrf.sig1) ∗
+  "%Heq" ∷ ⌜e.(evidVrf.vrfPk0) ≠ e.(evidVrf.vrfPk1)⌝.
+
+Lemma wish_evidVrf_sig_pred e pk :
+  wish_evidVrf e pk -∗
+  ¬ cryptoffi.is_sig_pk pk (sig_pred sigγ).
+Proof.
+  iIntros "@ #His_pk".
+  rewrite /ktcore.wish_VerifyVrfSig.
+  iNamedSuffix "Hwish0" "0".
+  iNamedSuffix "Hwish1" "1".
+  iDestruct (cryptoffi.is_sig_to_pred with "His_pk His_sig0") as "#HP0".
+  iDestruct (cryptoffi.is_sig_to_pred with "His_pk His_sig1") as "#HP1".
+  iDestruct "HP0" as "[H|H]"; [|by iNamed "H"].
+  iNamedSuffix "H" "0".
+  iDestruct "HP1" as "[H|H]"; [|by iNamed "H"].
+  iNamedSuffix "H" "1".
+  (* stuck knowing that physical and logical vrfPk's match.
+  need to know that logical vrfPk has w64 length. *)
+Admitted.
+
+Lemma wp_evidVrf_check ptr_e e sl_pk pk :
+  {{{
+    is_pkg_init client ∗
+    "#Hown_evid" ∷ evidVrf.own ptr_e e (□) ∗
+    "#Hsl_pk" ∷ sl_pk ↦*□ pk
+  }}}
+  ptr_e @ (ptrT.id client.evidVrf.id) @ "check" #sl_pk
+  {{{
+    (err : bool), RET #err;
+    "Hgenie" ∷
+      match err with
+      | true => ¬ wish_evidVrf e pk
+      | false =>
+        "#Hwish_evidVrf" ∷ wish_evidVrf e pk
+      end
+  }}}.
+Proof.
+  wp_start as "@".
+  iNamed "Hown_evid".
+  wp_auto.
+  wp_apply ktcore.wp_VerifyVrfSig as "* @".
+  { iFrame "#". }
+  wp_if_destruct.
+  { iApply "HΦ". iIntros "@". by iApply "Hgenie". }
+  iNamedSuffix "Hgenie" "0".
+  wp_apply ktcore.wp_VerifyVrfSig as "* @".
+  { iFrame "#". }
+  wp_if_destruct.
+  { iApply "HΦ". iIntros "@". by iApply "Hgenie". }
+  iNamedSuffix "Hgenie" "1".
+  wp_apply bytes.wp_Equal as "_".
+  { iFrame "#". }
+  iApply "HΦ".
+  case_bool_decide.
+  - by iIntros "@".
+  - by iFrame "#".
+Qed.
+
+Definition wish_evidLink e pk : iProp Σ :=
+  "#Hwish0" ∷ ktcore.wish_VerifyLinkSig pk e.(evidLink.epoch) e.(evidLink.link0) e.(evidLink.sig0) ∗
+  "#Hwish1" ∷ ktcore.wish_VerifyLinkSig pk e.(evidLink.epoch) e.(evidLink.link1) e.(evidLink.sig1) ∗
+  "%Heq" ∷ ⌜e.(evidLink.link0) ≠ e.(evidLink.link1)⌝.
+
+Lemma wish_evidLink_sig_pred e pk :
+  wish_evidLink e pk -∗
+  ¬ cryptoffi.is_sig_pk pk (sig_pred sigγ).
+Proof. Admitted.
+
+Lemma wp_evidLink_check ptr_e e sl_pk pk :
+  {{{
+    is_pkg_init client ∗
+    "#Hown_evid" ∷ evidLink.own ptr_e e (□) ∗
+    "#Hsl_pk" ∷ sl_pk ↦*□ pk
+  }}}
+  ptr_e @ (ptrT.id client.evidLink.id) @ "check" #sl_pk
+  {{{
+    (err : bool), RET #err;
+    "Hgenie" ∷
+      match err with
+      | true => ¬ wish_evidLink e pk
+      | false =>
+        "#Hwish_evidLink" ∷ wish_evidLink e pk
+      end
+  }}}.
+Proof.
+  wp_start as "@".
+  iNamed "Hown_evid".
+  wp_auto.
+  wp_apply ktcore.wp_VerifyLinkSig as "* @".
+  { iFrame "#". }
+  wp_if_destruct.
+  { iApply "HΦ". iIntros "@". by iApply "Hgenie". }
+  iNamedSuffix "Hgenie" "0".
+  wp_apply ktcore.wp_VerifyLinkSig as "* @".
+  { iFrame "#". }
+  wp_if_destruct.
+  { iApply "HΦ". iIntros "@". by iApply "Hgenie". }
+  iNamedSuffix "Hgenie" "1".
+  wp_apply bytes.wp_Equal as "_".
+  { iFrame "#". }
+  iApply "HΦ".
+  case_bool_decide.
+  - by iIntros "@".
+  - by iFrame "#".
+Qed.
+
+Definition wish_Evid e pk : iProp Σ :=
+  match e.(Evid.vrf), e.(Evid.link) with
+  | Some e', None => wish_evidVrf e' pk
+  | None, Some e' => wish_evidLink e' pk
+  | _, _ => False
+  end.
+
+Lemma wish_Evid_sig_pred e pk :
+  wish_Evid e pk -∗
+  ¬ cryptoffi.is_sig_pk pk (sig_pred sigγ).
+Proof. Admitted.
+
+Lemma wp_Evid_Check ptr_e e sl_pk pk :
+  {{{
+    is_pkg_init client ∗
+    "#Hown_evid" ∷ Evid.own ptr_e e (□) ∗
+    "#Hsl_pk" ∷ sl_pk ↦*□ pk
+  }}}
+  ptr_e @ (ptrT.id client.Evid.id) @ "Check" #sl_pk
+  {{{
+    (err : bool), RET #err;
+    "Hgenie" ∷
+      match err with
+      | true => ¬ wish_Evid e pk
+      | false =>
+        "#Hwish_Evid" ∷ wish_Evid e pk
+      end
+  }}}.
+Proof.
+  wp_start as "@".
+  iNamed "Hown_evid".
+  wp_auto.
+  destruct e. simpl.
+
+  wp_if_destruct.
+  2: {
+    destruct vrf.
+    2: { by iDestruct "Hown_vrf" as "%". }
+    wp_if_destruct.
+    2: {
+      destruct link.
+      2: { by iDestruct "Hown_link" as "%". }
+      by iApply "HΦ". }
+    destruct link.
+    { iNamedSuffix "Hown_link" "'".
+      by iDestruct (typed_pointsto_not_null with "Hstruct'") as %?. }
+    wp_apply wp_evidVrf_check as "* @".
+    { iFrame "#". }
+    by iApply "HΦ". }
+
+  destruct vrf.
+  { iNamedSuffix "Hown_vrf" "'".
+    by iDestruct (typed_pointsto_not_null with "Hstruct'") as %?. }
+  wp_if_destruct.
+  { destruct link.
+    { iNamedSuffix "Hown_link" "'".
+      by iDestruct (typed_pointsto_not_null with "Hstruct'") as %?. }
+    by iApply "HΦ". }
+  destruct link.
+  2: { by iDestruct "Hown_link" as "%". }
+  wp_apply wp_evidLink_check as "* @".
+  { iFrame "#". }
+  by iApply "HΦ".
+Qed.
 
 End proof.
 End client.
